Remove TLocInfo

rocq-skylabs-brick/theories/lang/cpp/logic/initializers.v
@@ -136,7 +136,6 @@ Definition default_initialize_body `{Σ : cpp_logic, σ : genv}
   | Tresult_unop _ _ | Tresult_binop _ _ _
   | Tresult_call _ _ | Tresult_member_call _ _ _
   | Tresult_member _ _ | Tresult_parenlist _ _ => ERROR "default initialization requires a runtime type, got unresolved type"
-  | TLocInfo _ ty => default_initialize ty p Q
   end%pstring%I.
 
 mlock
@@ -223,8 +222,6 @@ Section default_initialize.
     { (* qualifiers *)
       case_match; eauto.
       case_match; first by iMod "wp"; iExFalso; rewrite ERROR_elim.
-      iApply (IHty with "HQ wp"). }
-    { (* location information *)
       iApply (IHty with "HQ wp"). }
   Qed.
 
@@ -373,7 +370,6 @@ Definition wp_initialize_unqualified_body `{Σ : cpp_logic, σ : genv}
   let UNSUPPORTED := funI m => |={top}=>?u UNSUPPORTED m in
   if q_volatile cv then False%I
   else
-    let ty := drop_loc_info ty in
     match ty with
     | Tvoid =>
       (*
@@ -454,16 +450,14 @@ Definition wp_initialize_unqualified_body `{Σ : cpp_logic, σ : genv}
     | Tresult_call _ _ | Tresult_member_call _ _ _
     | Tresult_member _ _ | Tresult_parenlist _ _
     | Tauto => UNSUPPORTED (initializing_type ty init)
-    | TLocInfo _ _ => False%I (* unreachable *)
     end%I.
 
 mlock
-Definition wp_initialize_unqualified `{Σ : cpp_logic, σ : genv}
-    (tu : translation_unit) (ρ : region)
+Definition wp_initialize_unqualified `{Σ : cpp_logic, σ : genv} :
+  ∀ (tu : translation_unit) (ρ : region)
     (cv : type_qualifiers) (ty : decltype)
-    (addr : ptr) (init : Expr) (Q : FreeTemps -> epred) : mpred :=
-  Cbn (Reduce (wp_initialize_unqualified_body fupd_compatible)
-    tu ρ cv ty addr init Q).
+    (addr : ptr) (init : Expr) (Q : FreeTemps -> epred), mpred :=
+  Cbn (Reduce (wp_initialize_unqualified_body fupd_compatible)).
 
 Definition wp_initialize `{Σ : cpp_logic, σ : genv} (tu : translation_unit) (ρ : region)
     (qty : decltype) (addr : ptr) (init : Expr) (Q : FreeTemps -> epred) : mpred :=
@@ -477,42 +471,41 @@ Lemma wp_initialize_unqualified_well_typed `{Σ : cpp_logic, σ : genv}
       wp_initialize_unqualified tu ρ cv ty addr init (fun free => reference_to (to_heap_type ty) addr -* Q free)
   |-- wp_initialize_unqualified tu ρ cv ty addr init Q.
 Proof.
-  revert cv addr init Q.
-  induction ty; intros; rewrite wp_initialize_unqualified.unlock; cbn.
-  all: try (case_match; subst; eauto).
+  rewrite wp_initialize_unqualified.unlock.
+  case_match; eauto.
+  case_match; subst; eauto.
   all: try (iApply wp_operand_frame; [ done | ];
     iIntros (??) "X Y";
-    iDestruct (observe (reference_to _ _) with "Y") as "#R";
-    iApply ("X" with "Y"); iFrame "#").
-  all: try (iApply wp_glval_frame; [ done | ];
-      iIntros (??) "X Y";
-      iDestruct (observe (reference_to _ _) with "Y") as "#?";
-      iApply ("X" with "Y"); rewrite /to_heap_type/=; done).
-  all: try (iApply wp_xval_frame; [ done | ];
-      iIntros (??) "X Y";
-      iDestruct (observe (reference_to _ _) with "Y") as "#?";
-      iApply ("X" with "Y"); rewrite /to_heap_type/=; done).
-  all: try (iApply wp_operand_frame; [ done | ];
-    iIntros (??) "[$ X] Y";
     iDestruct (observe (reference_to _ _) with "Y") as "#?";
-    iApply ("X" with "Y"); eauto).
-  all: try (case_bool_decide; eauto;
-    etransitivity; [ | apply wp_init_well_typed ];
-    iApply wp_init_frame; [ done | ];
-    iIntros (?) "X Y"; iApply "X";
-    rewrite /to_heap_type/=;
-    rewrite reference_to_erase/=/tqualified';
-    destruct cv; simpl; eauto).
-  all: try (etransitivity; [ | apply wp_init_well_typed ];
-    iApply wp_init_frame; [ done | ];
-    iIntros (?) "X Y"; iApply "X";
-    rewrite (reference_to_erase (Tnamed gn));
-    rewrite reference_to_erase/=/tqualified';
-    destruct cv; simpl; eauto).
-  specialize (IHty cv addr init Q).
-  rewrite wp_initialize_unqualified.unlock H /= in IHty.
-  change (to_heap_type (TLocInfo l ty)) with (to_heap_type ty).
-  exact IHty.
+    iApply ("X" with "Y");
+    rewrite -reference_to_erase; done).
+  - iApply wp_glval_frame; [ done | ];
+      iIntros (??) "X Y";
+      iDestruct (observe (reference_to _ _) with "Y") as "#?".
+      iApply ("X" with "Y"). rewrite /to_heap_type/=. done.
+  - iApply wp_xval_frame; [ done | ];
+      iIntros (??) "X Y";
+      iDestruct (observe (reference_to _ _) with "Y") as "#?";
+      iApply ("X" with "Y").
+    rewrite /to_heap_type/=. done.
+  - iApply wp_operand_frame; [ done | ].
+    iIntros (??) "[$ X] Y".
+    iDestruct (observe (reference_to _ _) with "Y") as "#?";
+    iApply ("X" with "Y"); eauto.
+  - (* arrays *)
+    case_bool_decide; eauto.
+    etransitivity; [ | apply wp_init_well_typed ].
+    iApply wp_init_frame; [ done | ].
+    iIntros (?) "X Y". iApply "X".
+    rewrite /to_heap_type/=.
+    rewrite reference_to_erase/=/tqualified'.
+    destruct cv; simpl; eauto.
+  - etransitivity; [ | apply wp_init_well_typed ].
+    iApply wp_init_frame; [ done | ].
+    iIntros (?) "X Y". iApply "X".
+    rewrite (reference_to_erase (Tnamed gn)).
+    rewrite reference_to_erase/=/tqualified'.
+    destruct cv; simpl; eauto.
 Qed.
 
 (**
@@ -548,14 +541,8 @@ Section wp_initialize.
 
   (** [wp_initialize_unqualified] *)
 
-  Lemma wp_initialize_unqualified_loc_info : forall tu ρ cv li ty obj e Q,
-    wp_initialize_unqualified tu ρ cv (TLocInfo li ty) obj e Q -|-
-    wp_initialize_unqualified tu ρ cv ty obj e Q.
-  Proof. by intros; rewrite !wp_initialize_unqualified.unlock. Qed.
-
   Lemma wp_initialize_unqualified_intro tu ρ cv ty obj e Q :
-    Cbn (Reduce wp_initialize_unqualified_body false)
-      tu ρ cv ty obj e Q
+    Cbn (Reduce wp_initialize_unqualified_body false) tu ρ cv ty obj e Q
     |-- wp_initialize_unqualified tu ρ cv ty obj e Q.
   Proof.
     rewrite wp_initialize_unqualified.unlock. destruct ty; auto.
@@ -578,9 +565,8 @@ Section wp_initialize.
 
   Lemma wp_initialize_unqualified_elim tu ρ cv ty obj e Q :
     wp_initialize_unqualified tu ρ cv ty obj e Q
-    |-- Cbn (Reduce wp_initialize_unqualified_body fupd_compatible)
-      tu ρ cv ty obj e Q.
-  Proof. destruct ty; rewrite !wp_initialize_unqualified.unlock; cbn; auto. Qed.
+    |-- Cbn (Reduce wp_initialize_unqualified_body fupd_compatible) tu ρ cv ty obj e Q.
+  Proof. by rewrite wp_initialize_unqualified.unlock. Qed.
 
   (**
   For value types, [wp_initialize -|- wp_operand].
@@ -595,7 +581,6 @@ Section wp_initialize.
   Vvoid] in [wp_initialize_unqualified]'s [Tvoid] case.
   *)
   Definition can_init (ty : type) (e : Expr) : bool :=
-    let ty := drop_loc_info (drop_qualifiers ty) in
     bool_decide (ty = Tvoid) ==>
     bool_decide (type_of e = Tvoid).
 
@@ -616,51 +601,32 @@ Section wp_initialize.
 
   Lemma wp_initialize_unqualified_intro_val tu ρ cv ty (addr : ptr) init Q :
     can_init ty init ->
-    ~~ has_qualifiers ty -> is_value_type ty ->
+    ~~ is_qualified ty -> is_value_type ty ->
     VAL_INIT false tu ρ cv ty addr init Q
     |-- wp_initialize_unqualified tu ρ cv ty addr init Q.
   Proof.
-    revert cv Q. induction ty; intros cv Q Hty Hnq Hval;
-      rewrite -wp_initialize_unqualified_intro.
-    all: case_match; eauto.
-    all: try solve [ inversion Hnq | inversion Hval | eauto ].
-    { (* void *)
-      iIntros "wp /=".
-      iApply wp_operand_well_typed.
-      iApply (wp_operand_wand with "wp"). iIntros (v f).
-      rewrite can_init_void// has_type_void. iIntros "HQ ->".
-      rewrite tptsto_fuzzyR_Vvoid_primR. by iFrame "HQ". }
-    { cbn in Hty, Hnq, Hval.
-      have IH := IHty cv Q Hty Hnq Hval.
-      rewrite H in IH. iIntros "wp".
-      have Helim := wp_initialize_unqualified_elim tu ρ cv ty addr init Q.
-      rewrite H /= in Helim. iApply Helim. iApply IH.
-      iApply (wp_operand_wand with "wp"). iIntros (v f) "HQ R".
-      iApply "HQ". iApply _at_tptsto_fuzzyR_loc_info_intro. iFrame. }
+    intros Hty ??. rewrite -wp_initialize_unqualified_intro.
+    case_match; eauto.
+    destruct ty; try solve [ inversion H0 | eauto ].
+    (* void *)
+    iIntros "wp /=".
+    iApply wp_operand_well_typed.
+    iApply (wp_operand_wand with "wp"). iIntros (v f).
+    rewrite can_init_void// has_type_void. iIntros "HQ ->".
+    rewrite tptsto_fuzzyR_Vvoid_primR. by iFrame "HQ".
   Qed.
 
   Lemma wp_initialize_unqualified_elim_val tu ρ cv ty addr init Q :
-    ~~ has_qualifiers ty -> is_value_type ty ->
+    ~~ is_qualified ty -> is_value_type ty ->
     wp_initialize_unqualified tu ρ cv ty addr init Q
     |-- VAL_INIT fupd_compatible tu ρ cv ty addr init Q.
   Proof.
-    revert cv Q. induction ty; intros cv Q Hnq Hval;
-      rewrite wp_initialize_unqualified_elim.
-    all: case_match; eauto.
-    all: try solve [ inversion Hnq | inversion Hval | eauto ].
-    { (* void *)
-      iIntros "wp".
-      iApply (wp_operand_wand with "wp"). iIntros (v f) "(-> & HQ) R".
-      iApply ("HQ" with "[R]"). cbn. by rewrite tptsto_fuzzyR_Vvoid_primR. }
-    { cbn in Hnq, Hval.
-      have IH := IHty cv Q Hnq Hval.
-      rewrite H in IH. iIntros "wp".
-      have Hintro := wp_initialize_unqualified_intro tu ρ cv ty addr init Q.
-      rewrite H /= in Hintro.
-      iDestruct (Hintro with "wp") as "wp".
-      iDestruct (IH with "wp") as "wp".
-      iApply (wp_operand_wand with "wp"). iIntros (v f) "HQ R".
-      iApply "HQ". iApply _at_tptsto_fuzzyR_loc_info_elim. iFrame. }
+    intros. rewrite wp_initialize_unqualified_elim.
+    case_match; eauto. destruct ty; try done.
+    (* void *)
+    iIntros "wp".
+    iApply (wp_operand_wand with "wp"). iIntros (v f) "(-> & HQ) R".
+    iApply ("HQ" with "[R]"). cbn. by rewrite tptsto_fuzzyR_Vvoid_primR.
   Qed.
 
   (**
@@ -671,34 +637,25 @@ Section wp_initialize.
     qty ≡ Tqualified cv ty -> is_aggregate_type ty ->
     wp_initialize_unqualified tu ρ cv ty addr init Q |-- wp_init tu ρ qty addr init Q.
   Proof.
-    revert qty. induction ty; intros qty Heq Hagg;
-      rewrite wp_initialize_unqualified_elim.
-    all: case_match; cbn [drop_loc_info]; [ iIntros "[]" | ].
-    all: try by rewrite ?(UNSUPPORTED_elim, bi.False_elim).
+    intros Heq ?. rewrite wp_initialize_unqualified_elim.
+    case_match; [ iIntros "[]" | ]; destruct ty; first
+      [ by rewrite ?(UNSUPPORTED_elim, bi.False_elim)
+      | idtac ].
     all: try by rewrite tqualified_equiv Heq.
-    have Heq' : qty ≡ Tqualified cv ty.
-    { etrans; first exact Heq. apply Tqualified_proper, TLocInfo_equiv. }
-    have Hintro := wp_initialize_unqualified_intro tu ρ cv ty addr init Q.
-    rewrite H /= in Hintro.
-    etransitivity; first exact Hintro.
-    apply IHty; [exact Heq' | exact Hagg].
+  (* Relevant to [fupd_compatible = true] in [wp_initialize]
+    (** Absurd cases *)
+    all: rewrite -fupd_wp_init; iMod 1; iExFalso; by rewrite ?UNSUPPORTED_elim.
+  *)
   Qed.
   Lemma wp_initialize_unqualified_intro_aggregate tu ρ cv ty qty addr init Q :
-    qty ≡ Tqualified cv ty -> ~~ has_qualifiers ty -> is_aggregate_type ty ->
+    qty ≡ Tqualified cv ty -> ~~ is_qualified ty -> is_aggregate_type ty ->
         (if q_volatile cv then False else wp_init tu ρ qty addr init Q)
     |-- wp_initialize_unqualified tu ρ cv ty addr init Q.
   Proof.
-    revert qty. induction ty; intros qty Heq Hnq Hagg;
-      rewrite -wp_initialize_unqualified_intro.
-    all: case_match; cbn [drop_loc_info]; [ iIntros "[]" | ].
-    all: try done.
-    all: try by rewrite tqualified_equiv Heq.
-    have Heq' : qty ≡ Tqualified cv ty.
-    { etrans; first exact Heq. apply Tqualified_proper, TLocInfo_equiv. }
-    etransitivity.
-    { apply IHty; [exact Heq' | exact Hnq | exact Hagg]. }
-    have Helim := wp_initialize_unqualified_elim tu ρ cv ty addr init Q.
-    by rewrite H /= in Helim.
+    intros Heq ??. rewrite -wp_initialize_unqualified_intro.
+    case_match; [ iIntros "[]" | ].
+    destruct ty; try done.
+    all: by rewrite tqualified_equiv Heq.
   Qed.
 
   (** Properties *)
@@ -708,9 +665,9 @@ Section wp_initialize.
     (Forall free, Q free -* Q' free)
     |-- wp_initialize_unqualified tu ρ cv ty obj e Q -* wp_initialize_unqualified tu' ρ cv ty obj e Q'.
   Proof.
-    intros. induction ty; iIntros "HQ'"; rewrite unlock; auto.
+    intros. iIntros "HQ'". destruct ty; rewrite unlock; auto.
     all: case_match; eauto.
-    all: try (
+    all:
       repeat case_match;
       lazymatch goal with
       | |- context [wp_operand] => iApply wp_operand_frame; [done|]
@@ -723,9 +680,9 @@ Section wp_initialize.
       first
         [ by iIntros (??) "HQ ?"; iApply "HQ'"; iApply "HQ"
         | by iIntros (?) "?"; iApply "HQ'"
-        | eauto ]).
+        | eauto ].
     (* void *)
-    all: try (iIntros (??) "($ & HQ) ?"; iApply "HQ'"; by iApply "HQ").
+    iIntros (??) "($ & HQ) ?". iApply "HQ'". by iApply "HQ".
   Qed.
 
   Lemma wp_initialize_unqualified_shift tu ρ cv ty obj e Q :
@@ -783,8 +740,7 @@ Section wp_initialize.
   Qed.
 
   Lemma wp_initialize_intro tu ρ ty addr init Q :
-    qual_norm (fun cv rty => Cbn (Reduce wp_initialize_unqualified_body false)
-      tu ρ cv rty addr init Q) ty
+    qual_norm (fun cv rty => Cbn (Reduce wp_initialize_unqualified_body false) tu ρ cv rty addr init Q) ty
     |-- wp_initialize tu ρ ty addr init Q.
   Proof.
     rewrite qual_norm_decompose_type wp_initialize_decompose_type.
@@ -793,8 +749,7 @@ Section wp_initialize.
 
   Lemma wp_initialize_elim tu ρ ty addr init Q :
     wp_initialize tu ρ ty addr init Q
-    |-- qual_norm (fun cv rty => Cbn (Reduce wp_initialize_unqualified_body fupd_compatible)
-      tu ρ cv rty addr init Q) ty.
+    |-- qual_norm (fun cv rty => Cbn (Reduce wp_initialize_unqualified_body fupd_compatible) tu ρ cv rty addr init Q) ty.
   Proof.
     rewrite wp_initialize_decompose_type qual_norm_decompose_type.
     apply wp_initialize_unqualified_elim.
@@ -812,7 +767,7 @@ Section wp_initialize.
     rewrite drop_qualifiers_decompose_type.
     rewrite is_value_type_decompose_type wp_initialize_decompose_type.
     rewrite qual_norm_decompose_type erase_qualifiers_decompose_type.
-    have := has_qualifiers_decompose_type ty. cbn. intros.
+    have := is_qualified_decompose_type (type_of init). cbn. intros.
     by rewrite -wp_initialize_unqualified_intro_val.
   Qed.
 
@@ -823,7 +778,7 @@ Section wp_initialize.
   Proof.
     rewrite is_value_type_decompose_type wp_initialize_decompose_type.
     rewrite qual_norm_decompose_type erase_qualifiers_decompose_type.
-    have := has_qualifiers_decompose_type ty.
+    have := is_qualified_decompose_type ty.
     apply wp_initialize_unqualified_elim_val.
   Qed.
 
@@ -841,10 +796,9 @@ Section wp_initialize.
     TCEq (is_volatile ty) false ->
     wp_init tu ρ ty addr init Q |-- wp_initialize tu ρ ty addr init Q.
   Proof.
-    have Hnq := has_qualifiers_decompose_type ty.
     rewrite is_aggregate_type_decompose_type wp_initialize_decompose_type.
     rewrite /decompose_type. intros.
-    rewrite -wp_initialize_unqualified_intro_aggregate; [| | exact Hnq | eauto ].
+    rewrite -wp_initialize_unqualified_intro_aggregate; [| | eauto | eauto ].
     { have->: q_volatile (qual_norm (fun cv t => (cv,t)) ty).1 = false.
       { rewrite 2!qual_norm_map. simpl. inversion H0. done. }
       reflexivity. }
@@ -856,17 +810,18 @@ Section wp_initialize.
     (Forall free, Q free -* Q' free)
     |-- wp_initialize tu ρ ty obj e Q -* wp_initialize tu' ρ ty obj e Q'.
   Proof.
-    intros. rewrite !wp_initialize_decompose_type.
-    destruct (decompose_type ty); cbn.
-    exact: wp_initialize_unqualified_frame.
+    intros. rewrite /wp_initialize/qual_norm.
+    induction (wp_initialize_ok tu ρ ty); last done.
+    rewrite !qual_norm'_unqual//. exact: wp_initialize_unqualified_frame.
   Qed.
 
   Lemma wp_initialize_shift tu ρ ty obj e Q :
     Cbn (|={top}=>?fupd_compatible wp_initialize tu ρ ty obj e (fun free => |={top}=>?fupd_compatible Q free))
     |-- wp_initialize tu ρ ty obj e Q.
   Proof.
-    rewrite !wp_initialize_decompose_type.
-    destruct (decompose_type ty); cbn; done.
+    rewrite /wp_initialize/qual_norm.
+    induction (wp_initialize_ok tu ρ ty); last done.
+    rewrite !qual_norm'_unqual//.
   (* Relevant to [fupd_compatible = true]
     apply wp_initialize_unqualified_shift.
   *)
