rocq-skylabs-brick/theories/lang/cpp/logic/destroy.v
@@ -150,20 +150,6 @@ Section prim.
   Context `{Σ : cpp_logic, σ : genv}.
   Implicit Types (Q : epred).
 
-  Lemma wp_destroy_prim_loc_info : forall tu cv li ty (this : ptr) Q,
-    wp_destroy_prim tu cv (TLocInfo li ty) this Q -|-
-    wp_destroy_prim tu cv ty this Q.
-  Proof.
-    intros. rewrite !wp_destroy_prim.unlock /wp_destroy_prim_body /=.
-    iSplit.
-    - iIntros "H". iMod "H". iModIntro.
-      iDestruct "H" as "[H $]". iDestruct "H" as (v) "H". iExists v.
-      by iApply (_at_tptstoR_loc_info_elim with "H").
-    - iIntros "H". iMod "H". iModIntro.
-      iDestruct "H" as "[H $]". iDestruct "H" as (v) "H". iExists v.
-      by iApply (_at_tptstoR_loc_info_intro with "H").
-  Qed.
-
   Lemma wp_destroy_prim_intro tu cv ty (this : ptr) Q :
     (Exists v, this |-> tptstoR (erase_qualifiers ty) (cQp.mk (q_const cv) 1) v) ** Q
     |-- wp_destroy_prim tu cv ty this Q.
@@ -539,7 +525,6 @@ Section body.
       (cv : type_qualifiers) (rty : type) (this : ptr) (Q : epred) : mpred :=
     match rty with
     | Tqualified q ty => wp_destroy_val tu (merge_tq cv q) ty this Q
-    | TLocInfo _ ty => wp_destroy_val tu cv ty this Q
 
     | Tnamed cls =>
       |={top}=> |>
@@ -824,7 +809,6 @@ Section val_array.
     Let intro_body tu cv rty this Q : mpred :=
       match rty with
       | Tqualified q ty => wp_destroy_val tu (merge_tq cv q) ty this Q
-      | TLocInfo _ ty => wp_destroy_val tu cv ty this Q
       | Tnamed cls =>
         |>
         letI* := if q_const cv then wp_make_mutable tu this rty else id in
@@ -886,23 +870,6 @@ Section val_array.
     by rewrite wp_gen_succ.
   Qed.
 
-  Lemma wp_destroy_val_intro_val_unqual tu cv ty (this : ptr) Q :
-    ~~ has_qualifiers ty ->
-    is_value_type ty ->
-    (Exists v, this |-> tptstoR (erase_qualifiers ty)
-      (cQp.mk (q_const cv) 1) v) ** Q
-    |-- wp_destroy_val tu cv ty this Q.
-  Proof.
-    revert cv Q. induction ty; intros cv Q Hnq Hval;
-      rewrite -wp_destroy_val_intro /=; try done.
-    all: try (by rewrite -wp_destroy_prim_intro).
-    cbn [erase_qualifiers].
-    iIntros "[(%v & R) Q]".
-    iDestruct (_at_tptstoR_loc_info_elim with "R") as "R".
-    iApply (IHty cv Q); [assumption | assumption |].
-    iFrame.
-  Qed.
-
   Lemma wp_destroy_val_intro_val tu cv ty (this : ptr) Q :
     is_value_type ty ->
     let c := qual_norm' (fun cv _ => q_const cv) cv ty in
@@ -911,9 +878,10 @@ Section val_array.
   Proof.
     cbn. rewrite is_value_type_decompose_type erase_qualifiers_decompose_type.
     rewrite qual_norm'_decompose_type wp_destroy_val_decompose_type.
-    have := has_qualifiers_decompose_type ty.
+    have := is_qualified_decompose_type ty.
     destruct (decompose_type ty) as [cv' rty]; cbn=>??.
-    apply wp_destroy_val_intro_val_unqual; assumption.
+    rewrite -wp_destroy_val_intro. destruct rty; try done.
+    all: by rewrite -wp_destroy_prim_intro.
   Qed.
   Lemma destroy_val_intro_val tu ty (this : ptr) Q :
     is_value_type ty ->
@@ -921,10 +889,9 @@ Section val_array.
     (Exists v, this |-> tptstoR (erase_qualifiers ty) (cQp.mk (q_const cv) 1) v) ** Q
     |-- destroy_val tu ty this Q.
   Proof.
-    have Hnq := has_qualifiers_decompose_type ty.
     rewrite is_value_type_decompose_type qual_norm_decompose_type.
     rewrite erase_qualifiers_decompose_type destroy_val_decompose_type.
-    cbn. intros. by rewrite -wp_destroy_val_intro_val ?qual_norm'_unqual //.
+    cbn. intros. by rewrite -wp_destroy_val_intro_val ?qual_norm'_unqual.
   Qed.
 
   Lemma anyR_wp_destroy_val_val tu cv ty (this : ptr) Q :
@@ -944,24 +911,9 @@ Section val_array.
     this |-> anyR (erase_qualifiers ty) (cQp.mk (q_const cv) 1) ** Q
     |-- destroy_val tu ty this Q.
   Proof.
-    have Hnq := has_qualifiers_decompose_type ty.
     rewrite is_value_type_decompose_type qual_norm_decompose_type.
     rewrite erase_qualifiers_decompose_type destroy_val_decompose_type.
-    cbn. intros. by rewrite -anyR_wp_destroy_val_val ?qual_norm'_unqual //.
-  Qed.
-
-  Lemma wp_destroy_val_intro_ref_unqual tu cv ty (this : ptr) Q :
-    ~~ has_qualifiers ty ->
-    is_reference_type ty ->
-    (Exists v, this |-> tptstoR
-      (Tref $ erase_qualifiers $ syntax.types.as_ref ty)
-      (cQp.mk (q_const cv) 1) v) ** Q
-    |-- wp_destroy_val tu cv ty this Q.
-  Proof.
-    revert cv Q. induction ty; intros cv Q Hnq Href;
-      rewrite -wp_destroy_val_intro /=; try done.
-    all: try (by rewrite -wp_destroy_prim_intro).
-    apply IHty; assumption.
+    cbn. intros. by rewrite -anyR_wp_destroy_val_val ?qual_norm'_unqual.
   Qed.
 
   Lemma wp_destroy_val_intro_ref tu cv ty (this : ptr) Q :
@@ -972,9 +924,10 @@ Section val_array.
   Proof.
     cbn. rewrite is_reference_type_decompose_type as_ref_decompose_type.
     rewrite qual_norm'_decompose_type wp_destroy_val_decompose_type.
-    have := has_qualifiers_decompose_type ty.
+    have := is_qualified_decompose_type ty.
     destruct (decompose_type ty) as [cv' rty]; cbn=>??.
-    apply wp_destroy_val_intro_ref_unqual; assumption.
+    rewrite -wp_destroy_val_intro. destruct rty; try done.
+    all: by rewrite -wp_destroy_prim_intro.
   Qed.
 
   Lemma anyR_wp_destroy_val_ref tu cv ty (this : ptr) Q :
@@ -993,10 +946,9 @@ Section val_array.
     this |-> anyR (Tref $ erase_qualifiers $ as_ref ty) (cQp.mk (q_const cv) 1) ** Q
     |-- destroy_val tu ty this Q.
   Proof.
-    have Hnq := has_qualifiers_decompose_type ty.
     rewrite is_reference_type_decompose_type qual_norm_decompose_type.
     rewrite as_ref_decompose_type destroy_val_decompose_type.
-    cbn. intros. by rewrite -anyR_wp_destroy_val_ref ?qual_norm'_unqual //.
+    cbn. intros. by rewrite -anyR_wp_destroy_val_ref ?qual_norm'_unqual.
   Qed.
 
   Lemma anyR_wp_destroy_array tu cv ety n (p : ptr) Q :
@@ -1022,38 +974,27 @@ Section val_array.
     |-- Cbn (Reduce (V tu QM ty this Q)).
   Proof. by destroy_val_unfold. Qed.
 
-  Lemma wp_destroy_val_value_type_elim_unqual tu cv ty this Q :
-    ~~ has_qualifiers ty ->
-    is_value_type ty ->
-    wp_destroy_val tu cv ty this Q |-- wp_destroy_prim tu cv ty this Q.
-  Proof.
-    revert cv. induction ty; intros cv Hnq Hval;
-      wp_destroy_val_unfold; try done.
-    all: try reflexivity.
-    rewrite wp_destroy_prim_loc_info. apply IHty; assumption.
-  Qed.
-
   Lemma wp_destroy_val_value_type_elim tu cv ty this Q :
     is_value_type ty ->
     wp_destroy_val tu cv ty this Q |--
-      let p := decompose_type ty in
-      wp_destroy_prim tu (merge_tq cv p.1) p.2 this Q.
+      qual_norm' (fun cv ty =>
+        wp_destroy_prim tu cv ty this Q
+      ) cv ty.
   Proof.
-    rewrite wp_destroy_val_decompose_type is_value_type_decompose_type.
-    have Hnq := has_qualifiers_decompose_type ty.
-    destruct (decompose_type ty) as [cv' rty]; cbn; intros Hval.
-    apply wp_destroy_val_value_type_elim_unqual; assumption.
+    rewrite {1}wp_destroy_val_qual_norm'.
+    elim: (qual_norm'_ok _ cv ty); [|done]. move=>? rty *.
+    rewrite qual_norm'_unqual//. wp_destroy_val_unfold.
+    by destruct rty.
   Qed.
-
   Lemma destroy_val_value_type_elim tu ty this Q :
     is_value_type ty ->
     destroy_val tu ty this Q |--
-      let p := decompose_type ty in
-      wp_destroy_prim tu p.1 p.2 this Q.
+      qual_norm (fun cv ty =>
+        wp_destroy_prim tu cv ty this Q
+      ) ty.
   Proof.
-    intros Hval.
-    rewrite destroy_val_wp_destroy_val wp_destroy_val_value_type_elim //.
-    destruct (decompose_type ty); cbn. by rewrite left_id_L.
+    intros.
+    by rewrite destroy_val_wp_destroy_val  wp_destroy_val_value_type_elim.
   Qed.
 
   Lemma wp_destroy_array_elim tu cv ety n p Q :
