rocq-skylabs-brick/theories/lang/cpp/logic/heap_pred/any.v
@@ -34,10 +34,6 @@ Definition anyR `{Σ : cpp_logic} {σ : genv} (ty : Rtype) (q : cQp.t) : Rep :=
 Section with_cpp.
   Context `{Σ : cpp_logic} {σ : genv}.
 
-  Lemma anyR_loc_info li ty q :
-    anyR (TLocInfo li ty) q -|- anyR ty q.
-  Proof. by rewrite anyR.unlock !everywhereR_unfold /=. Qed.
-
   #[global] Instance anyR_timeless : ∀ ty q, Timeless (anyR ty q).
   Proof.
     intros. red.
@@ -96,8 +92,9 @@ Section with_cpp.
     { intros.
       iIntros "H".
       iDestruct (IHty with "H") as "%".
-      rewrite qualify_frac in H0.
-      eauto. }
+      { by erewrite zero_sized_array_qual. }
+      { rewrite qualify_frac in H0.
+        eauto. } }
   Qed.
 
   #[global] Instance anyR_as_fractional ty : AsCFractional0 (anyR ty).
@@ -115,15 +112,15 @@ Section with_cpp.
   Proof. by rewrite anyR.unlock everywhereR_Tqualified. Qed.
 
   #[local] Lemma not_heap_type (t : type) :
-    (if drop_loc_info t is Tqualified _ _ then false else
-       is_value_type (drop_loc_info t) || match drop_loc_info t with
+    (if t is Tqualified _ _ then false else
+       is_value_type t || match t with
                         | Tref _ => true
                         | _ => false
                         end) = false ->
     Is_true (is_heap_type t) -> False.
   Proof.
     rewrite /is_heap_type.
-    destruct (drop_loc_info t); try (move => ->; rewrite andb_false_r; inversion 1).
+    destruct t; try (move => ->; rewrite andb_false_r; inversion 1).
     intros. case_bool_decide; try inversion H0.
     by symmetry in H1; apply unqual_erase_qualifiers in H1.
   Qed.
@@ -139,7 +136,8 @@ Section with_cpp.
     all: try solve [
              intros;
              iIntros "H"; iDestruct (observe [| is_heap_type _ |] with "H") as "%H";
-             exfalso; revert H; rewrite /is_heap_type /=; naive_solver
+             exfalso; revert H;
+             apply not_heap_type; reflexivity
            | intros; rewrite anyR.unlock everywhereR_unfold/primitiveR/=; eauto ].
     { (* pointers *)
       iIntros (??) "H".
@@ -162,11 +160,6 @@ Section with_cpp.
       iExists v; iStopProof. f_equiv.
       rewrite /is_heap_type in H.
       case_bool_decide; auto. exfalso; done. }
-    { intros. iIntros "H".
-      iDestruct (observe [| is_heap_type _ |] with "H") as %Hheap.
-      exfalso; eapply (not_heap_type (Tqualified q t));
-        [ reflexivity | exact Hheap ]. }
-    { intros. rewrite tptstoR_loc_info anyR_loc_info. apply IHt. }
   Qed.
 
   Lemma anyR_tptstoR_val : ∀ t q,
@@ -197,11 +190,6 @@ Section with_cpp.
       rewrite decompose_type_qual/=.
       by rewrite qualify_merge_tq merge_tq_comm.
       Transparent decompose_type. }
-    { intros q Hv. rewrite anyR_loc_info.
-      rewrite /decompose_type qual_norm_unfold /=.
-      rewrite qual_norm'_decompose_pair /= left_id_L.
-      iIntros "H". iDestruct (IHt q Hv with "H") as (v) "R".
-      iExists v. rewrite tptstoR_loc_info. iFrame. }
   Qed.
   Lemma anyR_tptstoR_ref t q :
       anyR (Tref t) q -|- Exists v, tptstoR (Tref (erase_qualifiers t)) q v.
@@ -256,10 +244,7 @@ Section with_cpp.
     iIntros "H"; iExists _.
     iDestruct (observe [| is_heap_type _ |] with "H") as "%H".
     rewrite /is_heap_type in H.
-    case_bool_decide; auto.
-    { cbn in H0. injection H0 => ->.
-      rewrite erase_qualifiers_idemp. iFrame. }
-    { exfalso; done. }
+    case_bool_decide; auto. rewrite H0. eauto. exfalso; done.
   Qed.
 
   Lemma anyR_tptsto_fuzzyR_val_2 t q v :
