rocq-skylabs-brick/theories/lang/cpp/logic/pred.v
@@ -54,14 +54,10 @@ Definition pred_ns : namespace := nroot .@@ "skylabs" .@@ "lang" .@@ "cpp_logic"
 
 (* Used by [has_type_prop_has_type_noptr]. No theory. *)
 Definition nonptr_prim_type (ty : type) : bool :=
-  match drop_loc_info (drop_qualifiers ty) with
+  match drop_qualifiers ty with
   | Tfloat_ _ | Tchar_ _ | Tvoid | Tbool | Tenum _ | Tnum _ _ => true
   | Tnullptr | Tptr _ | Tref _ | Trv_ref _ | _ => false
   end.
-
-Lemma nonptr_prim_type_drop_qualifiers : forall (ty : type),
-    nonptr_prim_type ty = nonptr_prim_type (drop_qualifiers ty).
-Proof. induction ty; simpl; eauto. Qed.
 
 Lemma nonptr_prim_type_erase_qualifiers : forall (ty : type),
     nonptr_prim_type ty = nonptr_prim_type (erase_qualifiers ty).
@@ -190,8 +186,6 @@ Module Type CPP_LOGIC
          *)
       Axiom has_type_erase_qualifiers : ∀ ty v,
         has_type v ty -|- has_type v (erase_qualifiers ty).
-      Axiom has_type_loc_info : ∀ li ty v,
-        has_type v (TLocInfo li ty) -|- has_type v ty.
 
       (* Internal statements: *)
       Axiom has_type_nullptr' : ∀ p,
@@ -213,8 +207,6 @@ Module Type CPP_LOGIC
          [reference_to_elim] except for the issue with non-standard types. *)
       Axiom reference_to_erase : forall ty p,
           reference_to ty p -|- reference_to (erase_qualifiers ty) p.
-      Axiom reference_to_loc_info : forall li ty p,
-          reference_to (TLocInfo li ty) p -|- reference_to ty p.
 
       (** The introduction and elimination forms are not the same
           to avoid using [has_type] as types that are not C++ types.
@@ -291,9 +283,6 @@ Module Type CPP_LOGIC
     #[global] Declare Instance tptsto_valid_type
       : forall (t : Rtype) (q : cQp.t) (a : ptr) (v : val),
         Observe [| is_heap_type t |] (tptsto t q a v).
-
-    Axiom tptsto_loc_info : forall li ty q p v,
-      tptsto (TLocInfo li ty) q p v -|- tptsto ty q p v.
 
     Axiom tptsto_nonnull : forall {σ} ty q a,
       tptsto ty q nullptr a |-- False.
@@ -1469,7 +1458,6 @@ Section has_type.
     induction 1.
     { done. }
     { by rewrite -!has_type_qual_iff. }
-    { by rewrite !has_type_loc_info. }
     all: by rewrite !has_type_nonptr ?has_type_prop_raw_bytes_of_val.
   Qed.
 
@@ -1495,10 +1483,6 @@ Section has_type.
     by rewrite !has_type_or_undef_unfold -!has_type_qual_iff.
   Qed.
 
-  Lemma has_type_or_undef_loc_info li ty v :
-    has_type_or_undef v (TLocInfo li ty) -|- has_type_or_undef v ty.
-  Proof. by rewrite !has_type_or_undef_unfold has_type_loc_info. Qed.
-
   Lemma has_type_or_undef_val_related ty v1 v2 :
     val_related ty v1 v2 ->
     has_type_or_undef v1 ty |-- has_type_or_undef v2 ty.
@@ -1506,7 +1490,6 @@ Section has_type.
     induction 1.
     { done. }
     { by rewrite -!has_type_or_undef_qual_iff. }
-    { by rewrite !has_type_or_undef_loc_info. }
     all: rewrite !has_type_or_undef_nonundef//.
     all: by rewrite !has_type_nonptr// has_type_prop_raw_bytes_of_val.
   Qed.
