rocq-skylabs-brick/theories/lang/cpp/semantics/intensional.v
@@ -26,7 +26,6 @@ Fixpoint prim_initializable (t : type) : bool :=
   | Tbool
   | Tenum _
   | Tnullptr => true
-  | Tqualified _ t
-  | TLocInfo _ t => prim_initializable t
+  | Tqualified _ t => prim_initializable t
   | _ => false
   end.
