rocq-skylabs-brick/theories/lang/cpp/syntax/typing.v
@@ -22,12 +22,12 @@ Module decltype.
   on [to_valcat t] is simpler than matching on [t] when [t] might be
   an xvalue reference to a function type.
   *)
-  Definition to_exprtype_go (orig t : decltype) : ValCat * exprtype :=
-    match drop_loc_info (drop_qualifiers t) with
+  Definition to_exprtype (t : decltype) : ValCat * exprtype :=
+    match drop_qualifiers t with
     | Tref u => (Lvalue, u)
     | Trv_ref u =>
-      match as_function (drop_qualifiers u) with
-      | Some ft =>
+      match drop_qualifiers u with
+      | Tfunction _ as f =>
         (**
         Both "a function call or an overloaded operator expression,
         whose return type is rvalue reference to function" and "a cast
@@ -46,63 +46,12 @@ Module decltype.
         of "A function or reference type is always cv-unqualified."
         <https://www.eel.is/c++draft/basic.type.qualifier#1>
         *)
-        (Lvalue, Tfunction ft)
-      | None => (Xvalue, u)
+        (Lvalue, f)
+      | _ => (Xvalue, u)
       end
-    | _ => (Prvalue, orig)	(** Promote sharing, rather than normalize qualifiers *)
+    | _ => (Prvalue, t)	(** Promote sharing, rather than normalize qualifiers *)
     end.
-
-  Definition to_exprtype (t : decltype) : ValCat * exprtype :=
-    to_exprtype_go t t.
   Definition to_valcat (t : decltype) : ValCat := (to_exprtype t).1.
-
-  Lemma to_exprtype_go_tref orig q t :
-    (to_exprtype_go orig (tref q t)).1 = Lvalue.
-  Proof.
-    move: orig q. induction t; intros; rewrite /to_exprtype_go /=; auto;
-      apply IHt.
-  Qed.
-
-  Lemma to_valcat_tref q t : to_valcat (tref q t) = Lvalue.
-  Proof. apply to_exprtype_go_tref. Qed.
-
-  Lemma to_exprtype_go_nonref orig t :
-    ~~ is_reference_type t -> to_exprtype_go orig t = (Prvalue, orig).
-  Proof.
-    intros H. unfold to_exprtype_go, is_reference_type in *.
-    destruct (drop_loc_info (drop_qualifiers t)); simpl in *;
-      try contradiction; reflexivity.
-  Qed.
-
-  Lemma to_exprtype_nonref t :
-    ~~ is_reference_type t -> to_exprtype t = (Prvalue, t).
-  Proof. apply to_exprtype_go_nonref. Qed.
-
-  Lemma to_exprtype_go_reference orig t :
-    is_reference_type t -> (to_exprtype_go orig t).1 <> Prvalue.
-  Proof.
-    intros H. unfold to_exprtype_go, is_reference_type in *.
-    destruct (drop_loc_info (drop_qualifiers t)); simpl in *;
-      try contradiction; try discriminate.
-    destruct (as_function (drop_qualifiers t0)); discriminate.
-  Qed.
-
-  Lemma to_exprtype_reference t :
-    is_reference_type t -> (to_exprtype t).1 <> Prvalue.
-  Proof. apply to_exprtype_go_reference. Qed.
-
-  Lemma to_exprtype_go_prvalue_inv orig t u :
-    to_exprtype_go orig t = (Prvalue, u) -> orig = u.
-  Proof.
-    unfold to_exprtype_go.
-    destruct (drop_loc_info (drop_qualifiers t)); intros H; try discriminate;
-      try (inversion H; done).
-    destruct (as_function (drop_qualifiers t0)); discriminate.
-  Qed.
-
-  Lemma to_exprtype_prvalue_inv t u :
-    to_exprtype t = (Prvalue, u) -> t = u.
-  Proof. apply to_exprtype_go_prvalue_inv. Qed.
 
   (**
   Compute a declaration type from a value category and expression
@@ -136,17 +85,21 @@ Module decltype.
     Definition from_function_type (ft : function_type) : decltype :=
       normalize ft.(ft_return).
     Definition from_functype (t : functype) : M decltype :=
-      from_function_type <$> as_function t.
+      match t with
+      | Tfunction ft => mret $ from_function_type ft
+      | _ => mfail
+      end.
 
     Definition requireL (t : decltype) : M exprtype :=
-      match drop_loc_info (drop_qualifiers t) with
+      match drop_qualifiers t with
       | Tref t => mret t
       | _ => mfail
       end.
 
     Definition requireGL (t : decltype) : M exprtype :=
-      match drop_loc_info (drop_qualifiers t) with
-      | Tref t | Trv_ref t => mret t
+      match drop_qualifiers t with
+      | Tref t => mret t
+      | Trv_ref t => mret t
       | _ => mfail
       end.
 
@@ -162,7 +115,15 @@ Module decltype.
         | Cl2r_bitcast t => mret t
         | Cnoop t => mret t
         | Carray2ptr =>
-            let k cv base := Tptr <$> array_type_unqual cv base in
+            let k cv base :=
+              match base with
+              | Tarray ty _
+              | Tincomplete_array ty
+              | Tvariable_array ty _ =>
+                  mret $ Tptr $ tqualified cv ty
+              | _ => mfail
+              end
+            in
             requireGL base >>= qual_norm k
         | Cfun2ptr => Tptr <$> requireL base
         | Cint2ptr t
@@ -219,7 +180,10 @@ Module decltype.
 
       Definition of_call (f : Expr) : M decltype :=
         let* '(_, t) := to_exprtype <$> of_expr f in
-        unptr t >>= from_functype.
+        match t with
+        | Tptr ft => from_functype ft
+        | _ => mfail
+        end.
 
       Definition of_member (arrow : bool) (e : Expr) (mut : bool) (t : decltype) : M decltype :=
         let '(ref, et) := to_exprtype t in
@@ -229,13 +193,9 @@ Module decltype.
           let* '(lval, oty) :=
             let* et := to_exprtype <$> of_expr e in
             if arrow then
-              match et.1 with
-              | Prvalue =>
-                  match unptr et.2 with
-                  | Some t => mret (true, t)
-                  | None => mfail
-                  end
-              | _ => mfail
+              match et.1 , et.2 with
+              | Prvalue , Tptr t => mret (true, t)
+              | _ , _ => mfail
               end
             else
               match et.1 with
@@ -258,12 +218,10 @@ Module decltype.
             from_functype ft
         | inr e =>
             let* et := of_expr e in
-            let from_member_pointer et :=
-              match drop_loc_info (drop_qualifiers et) with
-              | Tmember_pointer _ ft => from_functype ft
-              | _ => mfail
-              end
-            in from_member_pointer et
+            match et with
+            | Tmember_pointer cls ft => from_functype ft
+            | _ => mfail
+            end
         end.
 
       Definition from_operator_impl (f : operator_impl) : M decltype :=
@@ -273,22 +231,14 @@ Module decltype.
         let* t1 := of_expr e1 in
         let* t2 := of_expr e2 in
         let arithmetic t := guard (Is_true $ is_arithmetic t) in
-        let subscript_operand vc ty other :=
-          match vc with
-          | Lvalue => const (tref QM) <$> arithmetic other <*> array_type ty
-          | Xvalue => const (trv_ref QM) <$> arithmetic other <*> array_type ty
-          | Prvalue =>
-              match unptr ty with
-              | Some ety => const (Tref ety) <$> arithmetic other
-              | None => mfail
-              end
-          end
-        in
-        let '(vc1, ty1) := to_exprtype t1 in
-        let '(vc2, ty2) := to_exprtype t2 in
-        match subscript_operand vc1 ty1 ty2 with
-        | Some ret => Some ret
-        | None => subscript_operand vc2 ty2 ty1
+        match drop_qualifiers t1 , drop_qualifiers t2 with
+        | Tref aty , other => const (tref QM) <$> arithmetic other <*> array_type aty
+        | Trv_ref aty , other => const (trv_ref QM) <$> arithmetic other <*> array_type aty
+        | Tptr ety , other => const (Tref ety) <$> arithmetic other
+        | other , Tref aty => const (tref QM) <$> arithmetic other <*> array_type aty
+        | other , Trv_ref aty => const (trv_ref QM) <$> arithmetic other <*> array_type aty
+        | other , Tptr ety => const (Tref ety) <$> arithmetic other
+        | _ , _ => mfail
         end.
 
       (**
@@ -304,19 +254,16 @@ Module decltype.
 
       #[local] Notation traverse_list := mapM.
 
-      Fixpoint cast_result_unqual (cv : type_qualifiers) (t : decltype) : decltype :=
-        match t with
-        | TLocInfo li t => TLocInfo li (cast_result_unqual cv t)
-        | Tnamed _
-        | Tarray _ _
-        | Tincomplete_array _
-        | Tvariable_array _ _
-        | Tenum _ => tqualified cv t
-        | _ => t
-        end.
-
       Definition cast_result : decltype -> decltype :=
-        qual_norm cast_result_unqual.
+        qual_norm (fun cv t =>
+          match t with
+          | Tnamed _
+          | Tarray _ _
+          | Tincomplete_array _
+          | Tvariable_array _ _
+          | Tenum _ => tqualified cv t
+          | _ => t
+          end).
 
       Definition of_expr_body (e : Expr) : M decltype :=
         match e return M decltype with
